src/PlutusIR/Analysis/BoundVars.v
@@ -116,25 +116,25 @@ Inductive appears_bound_in_tm (x : string) : term -> Prop :=
       appears_bound_in_tm x t ->
       appears_bound_in_tm x (Unwrap t)
 
-  | ABI_Tm_Constr_Cons_Head : forall i t ts,
+  | ABI_Tm_Constr_Cons_Head : forall i T t ts,
         appears_bound_in_tm x t ->
-        appears_bound_in_tm x (Constr i (t :: ts))
-  | ABI_Tm_Constr_Cons_Tail : forall i t ts,
-        appears_bound_in_tm x (Constr i ts) ->
-        appears_bound_in_tm x (Constr i (t :: ts))
-  | ABI_Tm_Constr_Nil : forall i t,
+        appears_bound_in_tm x (Constr i T (t :: ts))
+  | ABI_Tm_Constr_Cons_Tail : forall i T t ts,
+        appears_bound_in_tm x (Constr i T ts) ->
+        appears_bound_in_tm x (Constr i T (t :: ts))
+  | ABI_Tm_Constr_Nil : forall i t T,
         appears_bound_in_tm x t ->
-        appears_bound_in_tm x (Constr i (t :: nil))
+        appears_bound_in_tm x (Constr i T (t :: nil))
 
-  | ABI_Tm_Case_Cons_Tail : forall t t1 ts,
-        appears_bound_in_tm x (Case t ts) ->
-        appears_bound_in_tm x (Case t (t1 :: ts))
-  | ABI_Tm_Case_Cons_Head : forall t t1 ts,
+  | ABI_Tm_Case_Cons_Tail : forall T t t1 ts,
+        appears_bound_in_tm x (Case T t ts) ->
+        appears_bound_in_tm x (Case T t (t1 :: ts))
+  | ABI_Tm_Case_Cons_Head : forall T t t1 ts,
         appears_bound_in_tm x t1 ->
-        appears_bound_in_tm x (Case t (t1 :: ts))
-  | ABI_Tm_Case_Nil : forall t,
+        appears_bound_in_tm x (Case T t (t1 :: ts))
+  | ABI_Tm_Case_Nil : forall T t,
         appears_bound_in_tm x t ->
-        appears_bound_in_tm x (Case t nil)
+        appears_bound_in_tm x (Case T t nil)
 
   | ABI_Tm_Let_Nil : forall recty t0,
       appears_bound_in_tm x t0 ->
@@ -191,22 +191,24 @@ Inductive appears_bound_in_ann (X : string) : term -> Prop :=
       appears_bound_in_ann X t ->
       appears_bound_in_ann X (Unwrap t)
 
-  | ABI_Ann_Constr_Nil : forall i t,
+  | ABI_Ann_Constr_Nil : forall i T t,
+      appears_bound_in_ty X T ->
       appears_bound_in_ann X t ->
-      appears_bound_in_ann X (Constr i (t :: nil))
-  | ABI_Ann_Constr_Cons : forall i t ts,
-      appears_bound_in_ann X (Constr i ts) ->
-      appears_bound_in_ann X (Constr i (t :: ts))
+      appears_bound_in_ann X (Constr i T (t :: nil))
+  | ABI_Ann_Constr_Cons : forall i T t ts,
+      appears_bound_in_ann X (Constr i T ts) ->
+      appears_bound_in_ann X (Constr i T (t :: ts))
 
-  | ABI_Ann_Case_Cons_Head : forall t t1 ts,
-        appears_bound_in_ann X t1 ->
-        appears_bound_in_ann X (Case t (t1 :: ts))
-  | ABI_Ann_Case_Cons_Tail : forall t t1 ts,
-        appears_bound_in_ann X (Case t (t1 :: ts)) ->
-        appears_bound_in_ann X (Case t (t1 :: ts))
-  | ABI_Ann_Case_Nil : forall t,
-        appears_bound_in_ann X t ->
-        appears_bound_in_ann X (Case t [])
+  | ABI_Ann_Case_Cons_Head : forall T t t1 ts,
+      appears_bound_in_ann X t1 ->
+      appears_bound_in_ann X (Case T t (t1 :: ts))
+  | ABI_Ann_Case_Cons_Tail : forall T t t1 ts,
+      appears_bound_in_ann X (Case T t (t1 :: ts)) ->
+      appears_bound_in_ann X (Case T t (t1 :: ts))
+  | ABI_Ann_Case_Nil : forall T t,
+      appears_bound_in_ty X T ->
+      appears_bound_in_ann X t ->
+      appears_bound_in_ann X (Case T t [])
 
   | ABI_Ann_Error : forall T,
       appears_bound_in_ty X T ->
@@ -308,8 +310,8 @@ Function bound_vars (t : term) : list name :=
    | (Error ty)        => []
    | (Constant v)      => []
    | (Builtin f)       => []
-   | (Constr i ts)     => concat (map bound_vars ts)
-   | (Case t ts)       => bound_vars t ++ concat (map bound_vars ts)
+   | (Constr i T ts)   => concat (map bound_vars ts)
+   | (Case T t ts)     => bound_vars t ++ concat (map bound_vars ts)
    end
 with bound_vars_binding (b : binding) : list name := match b with
   | TermBind _ (VarDecl v _) t => [v] ++ bound_vars t
@@ -337,8 +339,8 @@ Fixpoint btv (t : term) : list tyname :=
    | Error ty        => Ty.btv ty
    | Constant v      => []
    | Builtin f       => []
-   | (Constr i ts)   => concat (map btv ts)
-   | (Case t ts)     => btv t ++ concat (map btv ts)
+   | (Constr i T ts) => concat (map btv ts)
+   | (Case T t ts)   => btv t ++ concat (map btv ts)
    end
 with btv_binding (b : binding) : list tyname := match b with
   | TermBind s (VarDecl v ty) t =>
