src/PlutusIR/Semantics/Dynamic/Datatypes.v
@@ -9,14 +9,19 @@ From PlutusCert Require Import
 
 Import ListNotations.
 
-
+(* Constructing constructor functions from their type signature *)
 
 (* Note [ Generating names ]
 
   Since on the term-level, the operational semantics never substitutes open
   terms, variable capture cannot happen.
-
 *)
+
+
+(* TODO compute SOP type from datatype declaration, when Ty_SOP is part of type
+ * language.
+ *)
+Axiom mk_SOP_ty : dtdecl -> ty.
 
 (* See note [Generating names] *)
 Definition mkName : nat -> string :=
@@ -24,27 +29,27 @@ Definition mkName : nat -> string :=
 .
 
 (* See constr_to_term *)
-Fixpoint constr_to_term_mono (ix : nat) (τ : ty) (n : nat) :=
-  match τ with
-    | Ty_Fun σ τ => LamAbs (mkName n) σ (constr_to_term_mono ix τ (S n))
-    | _          => Constr ix (map (Var ∘ mkName) (seq 0 n))
+Fixpoint constr_to_term_mono (ix : nat) (ty_sop : ty) (ty_constr : ty) (n : nat) :=
+  match ty_constr with
+    | Ty_Fun σ τ => LamAbs (mkName n) σ (constr_to_term_mono ix ty_sop τ (S n))
+    | _          => Constr ix ty_sop (map (Var ∘ mkName) (seq 0 n))
   end
 .
 
 
 
-(* Given a constructor with tag ix, type parameters α_0 .. α_n and type
+(* Given a constructor with tag ix, SOP type τ_SOP, type parameters α_0 .. α_n and type
  *
  *    σ_0 -> ... -> σ_n -> τ
  *
  * builds a term of the form:
  *
- *    Λ α_0. ... Λ α_1. λ0. ... λ n. Constr ix [0, ... n]
+ *    Λ α_0. ... Λ α_1. λ0. ... λ n. Constr ix τ_SOP [0, ... n]
  *)
-Fixpoint constr_to_term (ix : nat) (tyvars : list tvdecl) (τ : ty) :=
+Fixpoint constr_to_term (ix : nat) (ty_sop : ty) (tyvars : list tvdecl) (ty_constr : ty) :=
   match tyvars with
-    | []                      => constr_to_term_mono ix τ 0
-    | TyVarDecl α K :: tyvars => TyAbs α K (constr_to_term ix tyvars τ)
+    | []                      => constr_to_term_mono ix ty_sop ty_constr 0
+    | TyVarDecl α K :: tyvars => TyAbs α K (constr_to_term ix ty_sop tyvars ty_constr)
   end
 .
 
@@ -91,5 +96,8 @@ Definition dt_subst (dtd : dtdecl) : ty * term * list (string * term) :=
 
 Section Test.
   Open Scope string.
-  Compute (constr_to_term 3 [] (Ty_Fun (Ty_Var "a") (Ty_Fun (Ty_Var "b") (Ty_Var "c")))).
+
+  (* TODO: placeholder until Ty_SOP is part of type language *)
+  Definition ty_fake := Ty_Builtin DefaultUniInteger.
+  Compute (constr_to_term 3 ty_fake [] (Ty_Fun (Ty_Var "a") (Ty_Fun (Ty_Var "b") (Ty_Var "c")))).
 End Test.
